case-studies/kathrin/coq/Chapter9/girard.v
@@ -1,9 +1,9 @@
 (** * Appendix B: Strong Normalisation à la Girard *)
 
 Require Import core fintype.
-Import ScopedNotations.
 From Chapter9 Require Export preservation sn_raamsdonk.
 Open Scope fscope.
+Import ScopedNotations.
 
 (** ** Strong Normalisation *)
 Notation sn := (sn (@step _)).
